<?xml version="1.0" encoding="utf-8"?>
<rdf:RDF
   xmlns:cids="https://ontology.commonapproach.org/cids#"
   xmlns:dcterms="http://purl.org/dc/terms/"
   xmlns:foaf="http://xmlns.com/foaf/0.1/"
   xmlns:org="http://www.w3.org/ns/org#"
   xmlns:owl="http://www.w3.org/2002/07/owl#"
   xmlns:prov="http://www.w3.org/ns/prov#"
   xmlns:rdf="http://www.w3.org/1999/02/22-rdf-syntax-ns#"
   xmlns:rdfs="http://www.w3.org/2000/01/rdf-schema#"
   xmlns:skos="http://www.w3.org/2004/02/skos/core#"
   xmlns:vann="http://purl.org/vocab/vann/"
   xml:base="https://codelist.commonapproach.org/codeLists/PopulationServed#"
   xmlns="https://codelist.commonapproach.org/codeLists/PopulationServed#"
>
  <rdf:Description rdf:about="https://codelist.commonapproach.org/codeLists/PopulationServed">
    <rdf:type rdf:resource="http://www.w3.org/2002/07/owl#Ontology"/>
    <rdf:type rdf:resource="http://purl.org/vocommons/voafVocabulary"/>
    <vann:preferredNamespacePrefix>PopulationServed</vann:preferredNamespacePrefix>
    <owl:versionInfo>1.0</owl:versionInfo>
    <dcterms:date>08-10-2024</dcterms:date>
    <vann:preferredNamespaceUri rdf:resource="https://codelist.commonapproach.org/codeLists/PopulationServed#"/>
    <owl:imports rdf:resource="https://ontology.commonapproach.org/owl/cids"/>
    <owl:imports rdf:resource="http://www.w3.org/2006/time"/>
    <cids:hasName xml:lang="en">Population Served Codelist</cids:hasName>
    <dcterms:title xml:lang="en">Equity Deserving Groups</dcterms:title>
    <dcterms:description xml:lang="en">A codelist vocabulary of Populations Served.</dcterms:description>
    <foaf:name xml:lang="en">Population Served Codelist</foaf:name>
    <rdfs:label xml:lang="en">Population Served Codelist</rdfs:label>
    <dcterms:creator rdf:resource="https://ontology.commonapproach.org/cids#ac"/>
  </rdf:Description>

  <rdf:Description rdf:about="https://codelist.commonapproach.org/codeLists/PopulationServed#dataset">
    <rdf:type rdf:resource="http://www.w3.org/2004/02/skos/core#ConceptScheme"/>
  </rdf:Description>

  <rdf:Description rdf:about="#ps1">
    <rdf:type rdf:resource="https://ontology.commonapproach.org/cids#PopulationServed"/>
    <rdf:type rdf:resource="https://ontology.commonapproach.org/cids#CODE"/>
    <rdf:type rdf:resource="http://www.w3.org/2004/02/skos/core#Concept"/>
    <skos:inScheme rdf:resource="https://codelist.commonapproach.org/codeLists/PopulationServed#dataset"/>
    <rdfs:isDefinedBy rdf:resource="https://codelist.commonapproach.org/codeLists/PopulationServed#"/>
    <cids:hasName xml:lang="en">2SLGBTQIA+</cids:hasName>
    <rdfs:label xml:lang="en">2SLGBTQIA+</rdfs:label>
    <skos:definition xml:lang="en">People who identify as being two-spirit, lesbian, gay, bisexual, transgender, queer, intersex, asexual and others (“+”).</skos:definition>
    <cids:hasDefinition xml:lang="en">People who identify as being two-spirit, lesbian, gay, bisexual, transgender, queer, intersex, asexual and others (“+”).</cids:hasDefinition>
    <cids:definedBy rdf:resource="https://ontology.commonapproach.org/cids#ac"/>
    <cids:hasIdentifier>ps1</cids:hasIdentifier>
    <prov:hadPrimarySource rdf:resource="https://www.canada.ca/en/women-gender-equality/free-to-be-me/2slgbtqi-plus-glossary.html"/>
  </rdf:Description>

  <rdf:Description rdf:about="#ps2">
    <rdf:type rdf:resource="https://ontology.commonapproach.org/cids#PopulationServed"/>
    <rdf:type rdf:resource="https://ontology.commonapproach.org/cids#CODE"/>
    <rdf:type rdf:resource="http://www.w3.org/2004/02/skos/core#Concept"/>
    <skos:inScheme rdf:resource="https://codelist.commonapproach.org/codeLists/PopulationServed#dataset"/>
    <rdfs:isDefinedBy rdf:resource="https://codelist.commonapproach.org/codeLists/PopulationServed#"/>
    <cids:hasName xml:lang="en">Gender Diverse People: Agender</cids:hasName>
    <rdfs:label xml:lang="en">Gender Diverse People: Agender</rdfs:label>
    <skos:definition xml:lang="en">People who do not identify as, or with, any particular gender.</skos:definition>
    <cids:hasDefinition xml:lang="en">People who do not identify as, or with, any particular gender.</cids:hasDefinition>
    <cids:definedBy rdf:resource="https://ontology.commonapproach.org/cids#ac"/>
    <cids:hasIdentifier>ps2</cids:hasIdentifier>
    <prov:hadPrimarySource rdf:resource="https://dictionary.cambridge.org/dictionary/english/agender"/>
  </rdf:Description>


  <rdf:Description rdf:about="#ps3">
    <rdf:type rdf:resource="https://ontology.commonapproach.org/cids#PopulationServed"/>
    <rdf:type rdf:resource="https://ontology.commonapproach.org/cids#CODE"/>
    <rdf:type rdf:resource="http://www.w3.org/2004/02/skos/core#Concept"/>
    <skos:inScheme rdf:resource="https://codelist.commonapproach.org/codeLists/PopulationServed#dataset"/>
    <rdfs:isDefinedBy rdf:resource="https://codelist.commonapproach.org/codeLists/PopulationServed#"/>
    <cids:hasName xml:lang="en">Gender Diverse People: Non-Binary</cids:hasName>
    <rdfs:label xml:lang="en">Gender Diverse People: Non-Binary</rdfs:label>
    <skos:definition xml:lang="en">People whose gender identity does not align with a binary understanding of gender such as man or woman. It is a gender identity which may include man and woman, androgynous, fluid, multiple, no gender, or a different gender outside of the “woman—man” spectrum.</skos:definition>
    <cids:hasDefinition xml:lang="en">People whose gender identity does not align with a binary understanding of gender such as man or woman. It is a gender identity which may include man and woman, androgynous, fluid, multiple, no gender, or a different gender outside of the “woman—man” spectrum.</cids:hasDefinition>
    <cids:definedBy rdf:resource="https://ontology.commonapproach.org/cids#ac"/>
    <cids:hasIdentifier>ps3</cids:hasIdentifier>
    <prov:hadPrimarySource rdf:resource="https://www.canada.ca/en/women-gender-equality/free-to-be-me/2slgbtqi-plus-glossary.html"/>
  </rdf:Description>

  <rdf:Description rdf:about="#ps4">
    <rdf:type rdf:resource="https://ontology.commonapproach.org/cids#PopulationServed"/>
    <rdf:type rdf:resource="https://ontology.commonapproach.org/cids#CODE"/>
    <rdf:type rdf:resource="http://www.w3.org/2004/02/skos/core#Concept"/>
    <skos:inScheme rdf:resource="https://codelist.commonapproach.org/codeLists/PopulationServed#dataset"/>
    <rdfs:isDefinedBy rdf:resource="https://codelist.commonapproach.org/codeLists/PopulationServed#"/>
    <cids:hasName xml:lang="en">Gender Diverse People: Other</cids:hasName>
    <rdfs:label xml:lang="en">Gender Diverse People: Other</rdfs:label>
    <skos:definition xml:lang="en">People whose gender identity does not align with any of the other options provided.</skos:definition>
    <cids:hasDefinition xml:lang="en">People whose gender identity does not align with any of the other options provided.</cids:hasDefinition>
    <cids:definedBy rdf:resource="https://ontology.commonapproach.org/cids#ac"/>
    <cids:hasIdentifier>ps4</cids:hasIdentifier>
  </rdf:Description>

  <rdf:Description rdf:about="#ps5">
    <rdf:type rdf:resource="https://ontology.commonapproach.org/cids#PopulationServed"/>
    <rdf:type rdf:resource="https://ontology.commonapproach.org/cids#CODE"/>
    <rdf:type rdf:resource="http://www.w3.org/2004/02/skos/core#Concept"/>
    <skos:inScheme rdf:resource="https://codelist.commonapproach.org/codeLists/PopulationServed#dataset"/>
    <rdfs:isDefinedBy rdf:resource="https://codelist.commonapproach.org/codeLists/PopulationServed#"/>
    <cids:hasName xml:lang="en">Black People</cids:hasName>
    <rdfs:label xml:lang="en">Black People</rdfs:label>
    <skos:definition xml:lang="en">People belonging to any of various population groups of especially African ancestry often considered as having dark pigmentation of the skin but in fact having a wide range of skin colours.</skos:definition>
    <cids:hasDefinition xml:lang="en">People belonging to any of various population groups of especially African ancestry often considered as having dark pigmentation of the skin but in fact having a wide range of skin colours.</cids:hasDefinition>
    <cids:definedBy rdf:resource="https://ontology.commonapproach.org/cids#ac"/>
    <cids:hasIdentifier>ps5</cids:hasIdentifier>
    <prov:hadPrimarySource rdf:resource="https://www.noslangues-ourlanguages.gc.ca/en/publications/equite-diversite-inclusion-equity-diversity-inclusion-eng#notion-69399"/>
  </rdf:Description>


  <rdf:Description rdf:about="#ps6">
    <rdf:type rdf:resource="https://ontology.commonapproach.org/cids#PopulationServed"/>
    <rdf:type rdf:resource="https://ontology.commonapproach.org/cids#CODE"/>
    <rdf:type rdf:resource="http://www.w3.org/2004/02/skos/core#Concept"/>
    <skos:inScheme rdf:resource="https://codelist.commonapproach.org/codeLists/PopulationServed#dataset"/>
    <rdfs:isDefinedBy rdf:resource="https://codelist.commonapproach.org/codeLists/PopulationServed#"/>
    <cids:hasName xml:lang="en">Indigenous Peoples: First Nations</cids:hasName>
    <rdfs:label xml:lang="en">Indigenous Peoples: First Nations</rdfs:label>
    <skos:definition xml:lang="en">In Canada, Indigenous people who are part of a First Nation or whose ancestors were part of a First Nation. A First Nation person can be a Status or Non-Status Indian.</skos:definition>
    <cids:hasDefinition xml:lang="en">In Canada, Indigenous people who are part of a First Nation or whose ancestors were part of a First Nation. A First Nation person can be a Status or Non-Status Indian.</cids:hasDefinition>
    <cids:definedBy rdf:resource="https://ontology.commonapproach.org/cids#ac"/>
    <cids:hasIdentifier>ps6</cids:hasIdentifier>
    <prov:hadPrimarySource rdf:resource="https://www.noslangues-ourlanguages.gc.ca/en/publications/equite-diversite-inclusion-equity-diversity-inclusion-eng#notion-69399"/>
  </rdf:Description>


  <rdf:Description rdf:about="#ps7">
    <rdf:type rdf:resource="https://ontology.commonapproach.org/cids#PopulationServed"/>
    <rdf:type rdf:resource="https://ontology.commonapproach.org/cids#CODE"/>
    <rdf:type rdf:resource="http://www.w3.org/2004/02/skos/core#Concept"/>
    <skos:inScheme rdf:resource="https://codelist.commonapproach.org/codeLists/PopulationServed#dataset"/>
    <rdfs:isDefinedBy rdf:resource="https://codelist.commonapproach.org/codeLists/PopulationServed#"/>
    <cids:hasName xml:lang="en">Indigenous Peoples: Inuit</cids:hasName>
    <rdfs:label xml:lang="en">Indigenous Peoples: Inuit</rdfs:label>
    <skos:definition xml:lang="en">In Canada, Indigenous People that inhabit or that traditionally inhabited the northern regions and Arctic coasts of Canada known as Inuit Nunangat, and whose members are united by a common origin, history and culture.</skos:definition>
    <cids:hasDefinition xml:lang="en">In Canada, Indigenous People that inhabit or that traditionally inhabited the northern regions and Arctic coasts of Canada known as Inuit Nunangat, and whose members are united by a common origin, history and culture.</cids:hasDefinition>
    <cids:definedBy rdf:resource="https://ontology.commonapproach.org/cids#ac"/>
    <cids:hasIdentifier>ps7</cids:hasIdentifier>
    <prov:hadPrimarySource rdf:resource="https://www.noslangues-ourlanguages.gc.ca/en/publications/equite-diversite-inclusion-equity-diversity-inclusion-eng#notion-69399"/>
  </rdf:Description>

  <rdf:Description rdf:about="#ps8">
    <rdf:type rdf:resource="https://ontology.commonapproach.org/cids#PopulationServed"/>
    <rdf:type rdf:resource="https://ontology.commonapproach.org/cids#CODE"/>
    <rdf:type rdf:resource="http://www.w3.org/2004/02/skos/core#Concept"/>
    <skos:inScheme rdf:resource="https://codelist.commonapproach.org/codeLists/PopulationServed#dataset"/>
    <rdfs:isDefinedBy rdf:resource="https://codelist.commonapproach.org/codeLists/PopulationServed#"/>
    <cids:hasName xml:lang="en">Indigenous Peoples: Métis</cids:hasName>
    <rdfs:label xml:lang="en">Indigenous Peoples: Métis</rdfs:label>
    <skos:definition xml:lang="en">In Canada, Indigenous People whose members are of mixed First Nations and European ancestry, are united by a common origin, history and culture, and are generally accepted by the Métis Nation.</skos:definition>
    <cids:hasDefinition xml:lang="en">In Canada, Indigenous People whose members are of mixed First Nations and European ancestry, are united by a common origin, history and culture, and are generally accepted by the Métis Nation.</cids:hasDefinition>
    <cids:definedBy rdf:resource="https://ontology.commonapproach.org/cids#ac"/>
    <cids:hasIdentifier>ps8</cids:hasIdentifier>
    <prov:hadPrimarySource rdf:resource="https://www.noslangues-ourlanguages.gc.ca/en/publications/equite-diversite-inclusion-equity-diversity-inclusion-eng#notion-69399"/>
  </rdf:Description>

  <rdf:Description rdf:about="#ps9">
    <rdf:type rdf:resource="https://ontology.commonapproach.org/cids#PopulationServed"/>
    <rdf:type rdf:resource="https://ontology.commonapproach.org/cids#CODE"/>
    <rdf:type rdf:resource="http://www.w3.org/2004/02/skos/core#Concept"/>
    <skos:inScheme rdf:resource="https://codelist.commonapproach.org/codeLists/PopulationServed#dataset"/>
    <rdfs:isDefinedBy rdf:resource="https://codelist.commonapproach.org/codeLists/PopulationServed#"/>
    <cids:hasName xml:lang="en">Other Racialized Peoples</cids:hasName>
    <rdfs:label xml:lang="en">Other Racialized Peoples</rdfs:label>
    <skos:definition xml:lang="en">People other than Indigenous peoples or Black Canadians who are non-Caucasian in race or non-white in colour (refer to the Statistics Canada definition for “visible minorities”).</skos:definition>
    <cids:hasDefinition xml:lang="en">People other than Indigenous peoples or Black Canadians who are non-Caucasian in race or non-white in colour (refer to the Statistics Canada definition for “visible minorities”).</cids:hasDefinition>
    <cids:definedBy rdf:resource="https://ontology.commonapproach.org/cids#ac"/>
    <cids:hasIdentifier>ps9</cids:hasIdentifier>
  </rdf:Description>

  <rdf:Description rdf:about="#ps10">
    <rdf:type rdf:resource="https://ontology.commonapproach.org/cids#PopulationServed"/>
    <rdf:type rdf:resource="https://ontology.commonapproach.org/cids#CODE"/>
    <rdf:type rdf:resource="http://www.w3.org/2004/02/skos/core#Concept"/>
    <skos:inScheme rdf:resource="https://codelist.commonapproach.org/codeLists/PopulationServed#dataset"/>
    <rdfs:isDefinedBy rdf:resource="https://codelist.commonapproach.org/codeLists/PopulationServed#"/>
    <cids:hasName xml:lang="en">First Generation Immigrants, Refugees &amp; Newcomers</cids:hasName>
    <rdfs:label xml:lang="en">First Generation Immigrants, Refugees &amp; Newcomers</rdfs:label>
    <skos:definition xml:lang="en">People who were born outside Canada. For the most part, these are people who are now, or once were, immigrants to Canada. People who were forced to flee from persecution in their home country. This includes Convention refugees (as defined by the Immigration and Refugee Protection Act (S.C. 2001, c. 27)) and asylum-seekers or refugee claimants. Immigrants and Refugees that have been in Canada for less than five years.</skos:definition>
    <cids:hasDefinition xml:lang="en">People who were born outside Canada. For the most part, these are people who are now, or once were, immigrants to Canada. People who were forced to flee from persecution in their home country. This includes Convention refugees (as defined by the Immigration and Refugee Protection Act (S.C. 2001, c. 27)) and asylum-seekers or refugee claimants. Immigrants and Refugees that have been in Canada for less than five years.</cids:hasDefinition>
    <cids:definedBy rdf:resource="https://ontology.commonapproach.org/cids#ac"/>
    <cids:hasIdentifier>ps10</cids:hasIdentifier>
  </rdf:Description>

  <rdf:Description rdf:about="#ps11">
    <rdf:type rdf:resource="https://ontology.commonapproach.org/cids#PopulationServed"/>
    <rdf:type rdf:resource="https://ontology.commonapproach.org/cids#CODE"/>
    <rdf:type rdf:resource="http://www.w3.org/2004/02/skos/core#Concept"/>
    <skos:inScheme rdf:resource="https://codelist.commonapproach.org/codeLists/PopulationServed#dataset"/>
    <rdfs:isDefinedBy rdf:resource="https://codelist.commonapproach.org/codeLists/PopulationServed#"/>
    <cids:hasName xml:lang="en">Lone Parent Families</cids:hasName>
    <rdfs:label xml:lang="en">Lone Parent Families</rdfs:label>
    <skos:definition xml:lang="en">Families or homes where there is one parent present or living there. The lone, or single, parent can be any sex or gender, any ethnicity, and any sexuality. They do not have to be blood-related parents either to be classed as a parent.</skos:definition>
    <cids:hasDefinition xml:lang="en">Families or homes where there is one parent present or living there. The lone, or single, parent can be any sex or gender, any ethnicity, and any sexuality. They do not have to be blood-related parents either to be classed as a parent.</cids:hasDefinition>
    <cids:definedBy rdf:resource="https://ontology.commonapproach.org/cids#ac"/>
    <cids:hasIdentifier>ps11</cids:hasIdentifier>
  </rdf:Description>

  <rdf:Description rdf:about="#ps12">
    <rdf:type rdf:resource="https://ontology.commonapproach.org/cids#PopulationServed"/>
    <rdf:type rdf:resource="https://ontology.commonapproach.org/cids#CODE"/>
    <rdf:type rdf:resource="http://www.w3.org/2004/02/skos/core#Concept"/>
    <skos:inScheme rdf:resource="https://codelist.commonapproach.org/codeLists/PopulationServed#dataset"/>
    <rdfs:isDefinedBy rdf:resource="https://codelist.commonapproach.org/codeLists/PopulationServed#"/>
    <cids:hasName xml:lang="en">Northern Canadian Communities</cids:hasName>
    <rdfs:label xml:lang="en">Northern Canadian Communities</rdfs:label>
    <skos:definition xml:lang="en">Communities located, and people living, in Northern Canada, which is defined as: The three Canadian territories (Yukon, Northwest Territories, and Nunavut), and the northern extent of Newfoundland and Labrador, Quebec, Ontario, Manitoba, Saskatchewan, Alberta and British Columbia. North is based on provincially determined definitions that generally reflect administrative regions.</skos:definition>
    <cids:hasDefinition xml:lang="en">Communities located, and people living, in Northern Canada, which is defined as: The three Canadian territories (Yukon, Northwest Territories, and Nunavut), and the northern extent of Newfoundland and Labrador, Quebec, Ontario, Manitoba, Saskatchewan, Alberta and British Columbia. North is based on provincially determined definitions that generally reflect administrative regions.</cids:hasDefinition>
    <cids:definedBy rdf:resource="https://ontology.commonapproach.org/cids#ac"/>
    <cids:hasIdentifier>ps12</cids:hasIdentifier>
  </rdf:Description>

  <rdf:Description rdf:about="#ps13">
    <rdf:type rdf:resource="https://ontology.commonapproach.org/cids#PopulationServed"/>
    <rdf:type rdf:resource="https://ontology.commonapproach.org/cids#CODE"/>
    <rdf:type rdf:resource="http://www.w3.org/2004/02/skos/core#Concept"/>
    <skos:inScheme rdf:resource="https://codelist.commonapproach.org/codeLists/PopulationServed#dataset"/>
    <rdfs:isDefinedBy rdf:resource="https://codelist.commonapproach.org/codeLists/PopulationServed#"/>
    <cids:hasName xml:lang="en">Official Languages Minority Communities</cids:hasName>
    <rdfs:label xml:lang="en">Official Languages Minority Communities</rdfs:label>
    <skos:definition xml:lang="en">In Canada, official-language minority communities are mainly French-speaking people living outside the province of Quebec and English-speaking people living in the province of Quebec.</skos:definition>
    <cids:hasDefinition xml:lang="en">In Canada, official-language minority communities are mainly French-speaking people living outside the province of Quebec and English-speaking people living in the province of Quebec.</cids:hasDefinition>
    <cids:definedBy rdf:resource="https://ontology.commonapproach.org/cids#ac"/>
    <cids:hasIdentifier>ps13</cids:hasIdentifier>
  </rdf:Description>



  <rdf:Description rdf:about="#ps14">
    <rdf:type rdf:resource="https://ontology.commonapproach.org/cids#PopulationServed"/>
    <rdf:type rdf:resource="https://ontology.commonapproach.org/cids#CODE"/>
    <rdf:type rdf:resource="http://www.w3.org/2004/02/skos/core#Concept"/>
    <skos:inScheme rdf:resource="https://codelist.commonapproach.org/codeLists/PopulationServed#dataset"/>
    <rdfs:isDefinedBy rdf:resource="https://codelist.commonapproach.org/codeLists/PopulationServed#"/>
    <cids:hasName xml:lang="en">People Experiencing Homelessness or Housing Insecurities</cids:hasName>
    <rdfs:label xml:lang="en">People Experiencing Homelessness or Housing Insecurities</rdfs:label>
    <skos:definition xml:lang="en">People without stable, safe, permanent, appropriate housing, or the immediate prospect, means, and ability of acquiring it.</skos:definition>
    <cids:hasDefinition xml:lang="en">People without stable, safe, permanent, appropriate housing, or the immediate prospect, means, and ability of acquiring it.</cids:hasDefinition>
    <cids:definedBy rdf:resource="https://ontology.commonapproach.org/cids#ac"/>
    <cids:hasIdentifier>ps14</cids:hasIdentifier>
    <prov:hadPrimarySource rdf:resource="https://www.homelesshub.ca/sites/default/files/COHhomelessdefinition.pdf"/>
  </rdf:Description>

  <rdf:Description rdf:about="#ps15">
    <rdf:type rdf:resource="https://ontology.commonapproach.org/cids#PopulationServed"/>
    <rdf:type rdf:resource="https://ontology.commonapproach.org/cids#CODE"/>
    <rdf:type rdf:resource="http://www.w3.org/2004/02/skos/core#Concept"/>
    <skos:inScheme rdf:resource="https://codelist.commonapproach.org/codeLists/PopulationServed#dataset"/>
    <rdfs:isDefinedBy rdf:resource="https://codelist.commonapproach.org/codeLists/PopulationServed#"/>
    <cids:hasName xml:lang="en">People Living on Low Income</cids:hasName>
    <rdfs:label xml:lang="en">People Living on Low Income</rdfs:label>
    <skos:definition xml:lang="en">People living on low income as defined by any of several relative indicators/thresholds used by the Government of Canada to measure low income: low income cut-offs (LICOs), market basket measure (MBM), and/or low income measure (LIM).</skos:definition>
    <cids:hasDefinition xml:lang="en">People living on low income as defined by any of several relative indicators/thresholds used by the Government of Canada to measure low income: low income cut-offs (LICOs), market basket measure (MBM), and/or low income measure (LIM).</cids:hasDefinition>
    <cids:definedBy rdf:resource="https://ontology.commonapproach.org/cids#ac"/>
    <cids:hasIdentifier>ps15</cids:hasIdentifier>
    <prov:hadPrimarySource rdf:resource="https://www.canada.ca/en/employment-social-development/programs/poverty-reduction/backgrounder.html"/>
  </rdf:Description>


  <rdf:Description rdf:about="#ps16">
    <rdf:type rdf:resource="https://ontology.commonapproach.org/cids#PopulationServed"/>
    <rdf:type rdf:resource="https://ontology.commonapproach.org/cids#CODE"/>
    <rdf:type rdf:resource="http://www.w3.org/2004/02/skos/core#Concept"/>
    <skos:inScheme rdf:resource="https://codelist.commonapproach.org/codeLists/PopulationServed#dataset"/>
    <rdfs:isDefinedBy rdf:resource="https://codelist.commonapproach.org/codeLists/PopulationServed#"/>
    <cids:hasName xml:lang="en">People Living with Cognitive or Mental Health Related Issues</cids:hasName>
    <rdfs:label xml:lang="en">People Living with Cognitive or Mental Health Related Issues</rdfs:label>
    <skos:definition xml:lang="en">People living with disabilities, impairments, and/or functional limitations related to cognitive, learning, communication or mental health related issues, whether apparent or not, and permanent, temporary or episodic in nature, that hinders their full and equal participation in society when they face a barrier.</skos:definition>
    <cids:hasDefinition xml:lang="en">People living with disabilities, impairments, and/or functional limitations related to cognitive, learning, communication or mental health related issues, whether apparent or not, and permanent, temporary or episodic in nature, that hinders their full and equal participation in society when they face a barrier.</cids:hasDefinition>
    <cids:definedBy rdf:resource="https://ontology.commonapproach.org/cids#ac"/>
    <cids:hasIdentifier>ps16</cids:hasIdentifier>
    <prov:hadPrimarySource rdf:resource="https://laws-lois.justice.gc.ca/eng/acts/A-0.6/"/>
  </rdf:Description>


  <rdf:Description rdf:about="#ps17">
    <rdf:type rdf:resource="https://ontology.commonapproach.org/cids#PopulationServed"/>
    <rdf:type rdf:resource="https://ontology.commonapproach.org/cids#CODE"/>
    <rdf:type rdf:resource="http://www.w3.org/2004/02/skos/core#Concept"/>
    <skos:inScheme rdf:resource="https://codelist.commonapproach.org/codeLists/PopulationServed#dataset"/>
    <rdfs:isDefinedBy rdf:resource="https://codelist.commonapproach.org/codeLists/PopulationServed#"/>
    <cids:hasName xml:lang="en">People Living with Physical,Sensory or Pain Related Disabilities</cids:hasName>
    <rdfs:label xml:lang="en">People Living with Physical,Sensory or Pain Related Disabilities</rdfs:label>
    <skos:definition xml:lang="en">People living with disabilities, impairments, and/or functional limitations related to physical, sensory, or pain, whether apparent or not, and permanent, temporary or episodic in nature, that hinders their full and equal participation in society when they face a barrier.</skos:definition>
    <cids:hasDefinition xml:lang="en">People living with disabilities, impairments, and/or functional limitations related to physical, sensory, or pain, whether apparent or not, and permanent, temporary or episodic in nature, that hinders their full and equal participation in society when they face a barrier.</cids:hasDefinition>
    <cids:definedBy rdf:resource="https://ontology.commonapproach.org/cids#ac"/>
    <cids:hasIdentifier>ps17</cids:hasIdentifier>
    <prov:hadPrimarySource rdf:resource="https://laws-lois.justice.gc.ca/eng/acts/A-0.6/"/>
  </rdf:Description>

  <rdf:Description rdf:about="#ps18">
    <rdf:type rdf:resource="https://ontology.commonapproach.org/cids#PopulationServed"/>
    <rdf:type rdf:resource="https://ontology.commonapproach.org/cids#CODE"/>
    <rdf:type rdf:resource="http://www.w3.org/2004/02/skos/core#Concept"/>
    <skos:inScheme rdf:resource="https://codelist.commonapproach.org/codeLists/PopulationServed#dataset"/>
    <rdfs:isDefinedBy rdf:resource="https://codelist.commonapproach.org/codeLists/PopulationServed#"/>
    <cids:hasName xml:lang="en">People Living with Terminal or Chronic Illness/Diseases</cids:hasName>
    <rdfs:label xml:lang="en">People Living with Terminal or Chronic Illness/Diseases</rdfs:label>
    <skos:definition xml:lang="en">People living with disabilities, impairments, and/or functional limitations related to terminal or chronic illness/disease, whether apparent or not, and permanent, temporary or episodic in nature, that hinders their full and equal participation in society when they face a barrier.</skos:definition>
    <cids:hasDefinition xml:lang="en">People living with disabilities, impairments, and/or functional limitations related to terminal or chronic illness/disease, whether apparent or not, and permanent, temporary or episodic in nature, that hinders their full and equal participation in society when they face a barrier.</cids:hasDefinition>
    <cids:definedBy rdf:resource="https://ontology.commonapproach.org/cids#ac"/>
    <cids:hasIdentifier>ps18</cids:hasIdentifier>
    <prov:hadPrimarySource rdf:resource="https://laws-lois.justice.gc.ca/eng/acts/A-0.6/"/>
  </rdf:Description>

  <rdf:Description rdf:about="#ps19">
    <rdf:type rdf:resource="https://ontology.commonapproach.org/cids#PopulationServed"/>
    <rdf:type rdf:resource="https://ontology.commonapproach.org/cids#CODE"/>
    <rdf:type rdf:resource="http://www.w3.org/2004/02/skos/core#Concept"/>
    <skos:inScheme rdf:resource="https://codelist.commonapproach.org/codeLists/PopulationServed#dataset"/>
    <rdfs:isDefinedBy rdf:resource="https://codelist.commonapproach.org/codeLists/PopulationServed#"/>
    <cids:hasName xml:lang="en">People of Advanced Age (65+)</cids:hasName>
    <rdfs:label xml:lang="en">People of Advanced Age (65+)</rdfs:label>
    <skos:definition xml:lang="en">People who are 65 and older.</skos:definition>
    <cids:hasDefinition xml:lang="en">People who are 65 and older.</cids:hasDefinition>
    <cids:definedBy rdf:resource="https://ontology.commonapproach.org/cids#ac"/>
    <cids:hasIdentifier>ps19</cids:hasIdentifier>
  </rdf:Description>

  <rdf:Description rdf:about="#ps20">
    <rdf:type rdf:resource="https://ontology.commonapproach.org/cids#PopulationServed"/>
    <rdf:type rdf:resource="https://ontology.commonapproach.org/cids#CODE"/>
    <rdf:type rdf:resource="http://www.w3.org/2004/02/skos/core#Concept"/>
    <skos:inScheme rdf:resource="https://codelist.commonapproach.org/codeLists/PopulationServed#dataset"/>
    <rdfs:isDefinedBy rdf:resource="https://codelist.commonapproach.org/codeLists/PopulationServed#"/>
    <cids:hasName xml:lang="en">People without Advanced Educational Qualification</cids:hasName>
    <rdfs:label xml:lang="en">People without Advanced Educational Qualification</rdfs:label>
    <skos:definition xml:lang="en">People that have not completed any university, college or other post-secondary qualification.</skos:definition>
    <cids:hasDefinition xml:lang="en">People that have not completed any university, college or other post-secondary qualification.</cids:hasDefinition>
    <cids:definedBy rdf:resource="https://ontology.commonapproach.org/cids#ac"/>
    <cids:hasIdentifier>ps20</cids:hasIdentifier>
  </rdf:Description>

  <rdf:Description rdf:about="#ps21">
    <rdf:type rdf:resource="https://ontology.commonapproach.org/cids#PopulationServed"/>
    <rdf:type rdf:resource="https://ontology.commonapproach.org/cids#CODE"/>
    <rdf:type rdf:resource="http://www.w3.org/2004/02/skos/core#Concept"/>
    <skos:inScheme rdf:resource="https://codelist.commonapproach.org/codeLists/PopulationServed#dataset"/>
    <rdfs:isDefinedBy rdf:resource="https://codelist.commonapproach.org/codeLists/PopulationServed#"/>
    <cids:hasName xml:lang="en">Survivors of Domestic Violence, Sexual assault, Abuse or Stalking</cids:hasName>
    <rdfs:label xml:lang="en">Survivors of Domestic Violence, Sexual assault, Abuse or Stalking</rdfs:label>
    <skos:definition xml:lang="en">People who identify as being survivors of domestic violence, including intimate partner violence, sexual assault, stalking and/or harassment.</skos:definition>
    <cids:hasDefinition xml:lang="en">People who identify as being survivors of domestic violence, including intimate partner violence, sexual assault, stalking and/or harassment.</cids:hasDefinition>
    <cids:definedBy rdf:resource="https://ontology.commonapproach.org/cids#ac"/>
    <cids:hasIdentifier>ps21</cids:hasIdentifier>
  </rdf:Description>

  <rdf:Description rdf:about="#ps22">
    <rdf:type rdf:resource="https://ontology.commonapproach.org/cids#PopulationServed"/>
    <rdf:type rdf:resource="https://ontology.commonapproach.org/cids#CODE"/>
    <rdf:type rdf:resource="http://www.w3.org/2004/02/skos/core#Concept"/>
    <skos:inScheme rdf:resource="https://codelist.commonapproach.org/codeLists/PopulationServed#dataset"/>
    <rdfs:isDefinedBy rdf:resource="https://codelist.commonapproach.org/codeLists/PopulationServed#"/>
    <cids:hasName xml:lang="en">Women</cids:hasName>
    <rdfs:label xml:lang="en">Women</rdfs:label>
    <skos:definition xml:lang="en">All people who identify as women, whether they are cisgender or transgender women.</skos:definition>
    <cids:hasDefinition xml:lang="en">All people who identify as women, whether they are cisgender or transgender women.</cids:hasDefinition>
    <cids:definedBy rdf:resource="https://ontology.commonapproach.org/cids#ac"/>
    <cids:hasIdentifier>ps22</cids:hasIdentifier>
  </rdf:Description>
  
  <rdf:Description rdf:about="#ps23">
    <rdf:type rdf:resource="https://ontology.commonapproach.org/cids#PopulationServed"/>
    <rdf:type rdf:resource="https://ontology.commonapproach.org/cids#CODE"/>
    <rdf:type rdf:resource="http://www.w3.org/2004/02/skos/core#Concept"/>
    <skos:inScheme rdf:resource="https://codelist.commonapproach.org/codeLists/PopulationServed#dataset"/>
    <rdfs:isDefinedBy rdf:resource="https://codelist.commonapproach.org/codeLists/PopulationServed#"/>
    <cids:hasName xml:lang="en">Children (Ages 0-15)</cids:hasName>
    <rdfs:label xml:lang="en">Children (Ages 0-15)</rdfs:label>
    <skos:definition xml:lang="en">Any person aged 0-15.</skos:definition>
    <cids:hasDefinition xml:lang="en">Any person aged 0-15.</cids:hasDefinition>
    <cids:definedBy rdf:resource="https://ontology.commonapproach.org/cids#ac"/>
    <cids:hasIdentifier>ps23</cids:hasIdentifier>
  </rdf:Description>

  <rdf:Description rdf:about="#ps24">
    <rdf:type rdf:resource="https://ontology.commonapproach.org/cids#PopulationServed"/>
    <rdf:type rdf:resource="https://ontology.commonapproach.org/cids#CODE"/>
    <rdf:type rdf:resource="http://www.w3.org/2004/02/skos/core#Concept"/>
    <skos:inScheme rdf:resource="https://codelist.commonapproach.org/codeLists/PopulationServed#dataset"/>
    <rdfs:isDefinedBy rdf:resource="https://codelist.commonapproach.org/codeLists/PopulationServed#"/>
    <cids:hasName xml:lang="en">Youth (Ages 15-24)</cids:hasName>
    <rdfs:label xml:lang="en">Youth (Ages 15-24)</rdfs:label>
    <skos:definition xml:lang="en">Any person aged 15-24.</skos:definition>
    <cids:hasDefinition xml:lang="en">Any person aged 15-24.</cids:hasDefinition>
    <cids:definedBy rdf:resource="https://ontology.commonapproach.org/cids#ac"/>
    <cids:hasIdentifier>ps24</cids:hasIdentifier>
  </rdf:Description>


  <rdf:Description rdf:about="#ps25">
    <rdf:type rdf:resource="https://ontology.commonapproach.org/cids#PopulationServed"/>
    <rdf:type rdf:resource="https://ontology.commonapproach.org/cids#CODE"/>
    <rdf:type rdf:resource="http://www.w3.org/2004/02/skos/core#Concept"/>
    <skos:inScheme rdf:resource="https://codelist.commonapproach.org/codeLists/PopulationServed#dataset"/>
    <rdfs:isDefinedBy rdf:resource="https://codelist.commonapproach.org/codeLists/PopulationServed#"/>
    <cids:hasName xml:lang="en">General Population</cids:hasName>
    <rdfs:label xml:lang="en">General Population</rdfs:label>
    <cids:definedBy rdf:resource="https://ontology.commonapproach.org/cids#ac"/>
    <cids:hasIdentifier>ps25</cids:hasIdentifier>
  </rdf:Description>



</rdf:RDF>
